Defined size of loop as function, and simplified proofs.

theories/EHoare.v
@@ -114,46 +114,21 @@ Proof.
     firstorder eauto.
 Qed.
 
-Inductive loop_sizeR : forall {st c st'}, st =[ c ]=> st' -> nat -> Prop :=
-| LS_WhileFalse : forall b st c exef,
-    loop_sizeR (E_WhileFalse b st c exef) 0
-| LS_WhileTrue : forall st st' st'' b c pft exec exew n,
-    loop_sizeR exew n ->
-    loop_sizeR (E_WhileTrue st st' st'' b c pft exec exew) (S n)
-.
+Fixpoint loop_size {st c st'} (exe : st =[ c ]=> st') : nat :=
+  match exe with
+  | E_WhileTrue _ _ _ _ _ _ _ exew => S (loop_size exew)
+  | _ => 0
+  end.
 
 Definition loop_measureR b c (Q : Assertion)
            (st : state) (n : nat) : Prop :=
   (~ (exists st' (exe : st =[ WHILE b DO c END ]=> st'), Q st') -> n = 0) /\
-  (forall m st' (exe : st =[ WHILE b DO c END ]=> st'),
+  (forall st' (exe : st =[ WHILE b DO c END ]=> st'),
       Q st' ->
-      loop_sizeR exe m ->
-      (forall m' st'' (exe' : st =[ WHILE b DO c END ]=> st''),
+      (forall st'' (exe' : st =[ WHILE b DO c END ]=> st''),
           Q st'' ->
-          loop_sizeR exe' m' ->
-          m <= m') ->
-      n = m).
-
-Lemma loop_sizeR_ex : forall st b c st' (exe : st =[ WHILE b DO c END ]=> st'),
-    exists n, loop_sizeR exe n.
-Proof.
-  intros. remember (WHILE b DO c END)%imp as c' eqn:Heq.
-  induction exe; inversion Heq; subst.
-  - repeat econstructor.
-  - firstorder eauto. repeat econstructor. eauto.
-Qed.
-
-Lemma loop_sizeR_inv : forall st st' st'' b c pft pfc pfw n,
-    loop_sizeR (E_WhileTrue st st' st'' b c pft pfc pfw) n ->
-    exists m, loop_sizeR pfw m /\ S m = n.
-Proof.
-  intros until n. inversion 1.
-  repeat match goal with
-         | H : existT _ _ _ = existT _ _ _ |- _ =>
-           apply inj_pair2 in H; subst
-         end.
-  eauto.
-Qed.
+          loop_size exe <= loop_size exe') ->
+      n = loop_size exe).
 
 Lemma nonempty_smallest_ex (P : nat -> Prop) :
   (exists n, P n) ->
@@ -167,17 +142,19 @@ Qed.
 
 Lemma loop_measureR_ex b c Q st :
   (exists st' (exe : st =[ WHILE b DO c END ]=> st'), Q st') ->
-  exists m st' (exe : st =[ WHILE b DO c END ]=> st'),
-    Q st' /\ loop_sizeR exe m /\
-    (forall m' st'' (exe' : st =[ WHILE b DO c END ]=> st''),
-        Q st'' -> loop_sizeR exe' m' -> m <= m').
+  exists st' (exe : st =[ WHILE b DO c END ]=> st'),
+    Q st' /\
+    (forall st'' (exe' : st =[ WHILE b DO c END ]=> st''),
+        Q st'' -> loop_size exe <= loop_size exe').
 Proof.
   intros.
   edestruct (nonempty_smallest_ex
                (fun m => exists st' (exe : st =[ WHILE b DO c END ]=> st'),
-                    Q st' /\ loop_sizeR exe m)) as [m ?].
-  - destruct H as [? [H ?]]. edestruct loop_sizeR_ex with (exe:=H). eauto.
-  - destruct_conjs. exists m. repeat econstructor; eauto.
+                    Q st' /\ loop_size exe = m)).
+  - firstorder eauto.
+  - destruct_conjs. subst. repeat econstructor; eauto.
+    Grab Existential Variables.
+    auto.
 Qed.
 
 Lemma loop_measureR_is_fun b c Q : forall (st : state),
@@ -185,10 +162,12 @@ Lemma loop_measureR_is_fun b c Q : forall (st : state),
 Proof.
   unfold unique.
   intros. destruct (classic (exists st' (exe : st =[ WHILE b DO c END ]=> st'), Q st')) as [H | H].
-  - apply loop_measureR_ex in H. destruct H as [m ?]. destruct_conjs.
-    exists m. split.
+  - apply loop_measureR_ex in H. destruct H as [? [exe ?]]. destruct_conjs.
+    exists (loop_size exe). split.
     + split. intros. exfalso. eauto.
-      intros m'. intros. assert (m <= m') by eauto. assert (m' <= m) by eauto.
+      intros ? exe'. intros.
+      assert (loop_size exe <= loop_size exe') by eauto.
+      assert (loop_size exe' <= loop_size exe) by eauto.
       lia.
     + intros ? H'. destruct H' as [? H'].
       symmetry. eauto.
@@ -198,21 +177,20 @@ Proof.
       symmetry. eauto.
 Qed.
 
-Lemma loop_measureR_order : forall (Q : Assertion) st st' st'' b c pft exec exew m,
+Lemma loop_measureR_order : forall (Q : Assertion) st st' st'' b c pft exec exew,
     Q st'' ->
-    loop_sizeR (E_WhileTrue st st' st'' b c pft exec exew) m ->
-    (forall m' st''' (exe' : st =[ WHILE b DO c END ]=> st'''),
+    (forall st''' (exe' : st =[ WHILE b DO c END ]=> st'''),
         Q st''' ->
-        loop_sizeR exe' m' ->
-        m <= m') ->
-    forall m', loop_measureR b c Q st' m' ->
-          S m' = m.
+        loop_size (E_WhileTrue st st' st'' b c pft exec exew) <= loop_size exe') ->
+    forall m, loop_measureR b c Q st' m ->
+         S m = loop_size (E_WhileTrue st st' st'' b c pft exec exew).
 Proof.
-  intros until m. intros HQ Hs H m' H'. destruct H' as [_ H'].
-  apply loop_sizeR_inv in Hs. destruct Hs as [n [? ?]].
-  subst. f_equal. eapply H'; eauto.
-  intros. apply le_S_n.
-  eapply H; eauto. constructor. eauto.
+  intros until exew. intros HQ H m H'. destruct H' as [_ H'].
+  simpl loop_size in *. f_equal. eapply H'; eauto.
+  intros ? exe' ?.
+  apply le_S_n. etransitivity.
+  eapply (H _ (E_WhileTrue _ _ _ _ _ _ _ exe')); eauto.
+  simpl. eauto.
   Grab Existential Variables.
   all : eauto.
 Qed.
@@ -255,12 +233,12 @@ Proof.
       apply EH_While with (E:=measure).
       intros. apply IHc. intros. destruct_conjs. subst.
       destruct (Hm st) as [_ Hm'].
-      edestruct loop_measureR_ex as [m [st' [exe ?]]]; eauto. destruct_conjs.
+      edestruct loop_measureR_ex as [st' [exe ?]]; eauto. destruct_conjs.
       remember (WHILE b DO c END)%imp eqn:Heq.
       destruct exe; inversion Heq; subst; clear Heq. exfalso. congruence.
       exists st'. eexists; eauto. intuition eauto.
       eapply loop_measureR_order in Hm; eauto.
-      assert (measure st = m) by eauto. lia.
+      rewrite <- Hm' in Hm; eauto. lia.
     + eauto.
     + simpl. intros ? [H ?]. destruct H as [? [exe ?]].
       inversion exe; subst; eauto. exfalso. eauto.
